- Standard linear regression formula: 
\begin{equation}

    y_i=\boldsymbol{\beta_0} +\mathbf{x}_i^\prime \boldsymbol{\beta}+\epsilon_i, \quad i = 1, \ldots, n,
    \tag{1}
    \end{equation}

- Lasso estimator formula:
\begin{equation}
    \hat{\boldsymbol{\beta}}^{\text{LASSO}}=\underset{\boldsymbol{\beta}}{\arg \min}\sum_{i=1}^N (y_i-\beta_0-\sum_{j=1}^p x_{i j}\beta_j)^2
    \tag{2}
    \end{equation} 
    
    subject to 
    
    \begin{equation}
    \sum_{j=1}^{p}\left|\beta_{j}\right|\leq t
    \tag{3}
    \end{equation}
    
- Lasso estimator with penalty: 
\begin{equation}
    \begin{aligned}
    \hat{\boldsymbol{\beta}}^{\text{LASSO}} &=\underset{\boldsymbol{\beta}}{\arg \min}\left\{\frac{1}{2}\sum_{i=1}^N (y_i-\beta_0-\sum_{j=1}^p x_{i j}\beta_j)^2 +\lambda \left(\sum_{j=1}^p |\beta_j|\right)\right\}.\\
    \end{aligned}
    \tag{4}
    \end{equation}

- Data-driven penalty term: 
\begin{equation}
    \lambda=2c \sqrt{n} \phi^{-1} (\frac{1-\gamma}{2p})
    \tag{6}
    \end{equation}

- Lasso estimator with penalty and loadings: 
\begin{equation}
    \begin{aligned}
    \hat{\boldsymbol{\beta}}^{\text{LASSO}} &=\underset{\boldsymbol{\beta}}{\arg \min}\left\{\frac{1}{2}\sum_{i=1}^N (y_i-\beta_0-\sum_{j=1}^p x_{i j}\beta_j)^2 +\lambda \left(\sum_{j=1}^p |\beta_j|\eta_j\right)\right\}.\\
    \end{aligned}
    \tag{5}
    \end{equation}

